wip

src/compilation/ReserveClosStep.v
@@ -338,6 +338,44 @@ Proof using w_ex_is_xacq WFSC WF IMMCON.
 Qed.
 
 (* TODO: move *)
+Lemma iiord_fixed_reserve_step_minus_reserved
+  tl tc1 tc2 s
+  (NORES : action tl <> ta_reserve)
+  (SRES  : s ⊆₁ action ↓₁ (eq ta_reserve))
+  (STEP  : iiord_step G sc tl tc1 tc2) :
+  iiord_step G sc tl ((tc1 \₁ action ↓₁ (eq ta_reserve)) ∪₁ s)
+                     ((tc2 \₁ action ↓₁ (eq ta_reserve)) ∪₁ s).
+Proof using.
+  clear -STEP SRES NORES.
+  destruct tl as [ta a]. destruct ta.
+  4: { exfalso. apply NORES. desf. }
+  all: destruct STEP as [STEP [AA BB]].
+  all: split; splits.
+  all: try now eapply iord_coherent_equiv_wo_reserved; [|apply AA]; split; [|rewrite SRES]; basic_solver.
+  all: try now eapply iord_coherent_equiv_wo_reserved; [|apply BB]; split; [|rewrite SRES]; basic_solver.
+  all: apply seq_eqv_l in STEP; destruct STEP as [TT STEP].
+  all: apply seq_eqv_l; split.
+  all: try now intros [HH|HH]; [|now apply SRES in HH; inv HH]; apply TT; apply HH.
+  all: rewrite STEP.
+  all: split; unfolder; ins; desf; ins; splits; auto.
+Qed.
+
+(* TODO: move *)
+Add Parametric Morphism : iiord_step with signature
+  eq ==> eq ==> eq ==> set_equiv ==> set_equiv ==> iff as iiord_step_more.
+Proof using.
+  clear. intros G sc a b c BC d e DE.
+  split; intros [HH [AA BB]]; split; splits.
+  all: try now eapply iord_coherent_more; eauto.
+  all: try now eapply iord_coherent_more; (try symmetry); eauto.
+  all: apply seq_eqv_l in HH; destruct HH as [CC DD].
+  all: apply seq_eqv_l; split.
+  all: try (generalize BC DE CC DD; basic_solver). 
+  { now rewrite <- DE, <- BC. }
+  now rewrite DE, BC.
+Qed.
+
+(* TODO: move *)
 Lemma iiord_no_reserve_step_minus_reserved
   tl tc1 tc2
   (NORES : action tl <> ta_reserve)
@@ -346,17 +384,27 @@ Lemma iiord_no_reserve_step_minus_reserved
                      (tc2 \₁ action ↓₁ (eq ta_reserve)).
 Proof using.
   clear -STEP NORES.
+  apply iiord_fixed_reserve_step_minus_reserved with (s:=fun _ => False) in STEP; auto.
+  2: basic_solver.
+  eapply iiord_step_more; [..| eauto]; auto.
+  all: basic_solver.
+Qed.
+
+(* TODO: move *)
+Lemma iiord_step_fixed_reserved s tl tc1 tc2
+  (SRES : s ⊆₁ action ↓₁ (eq ta_reserve))
+  (STEP : iiord_step G sc tl tc1 tc2) :
+  (iiord_step G sc tl)^? ((tc1 \₁ action ↓₁ (eq ta_reserve)) ∪₁ s)
+                         ((tc2 \₁ action ↓₁ (eq ta_reserve)) ∪₁ s).
+Proof using.
+  clear -STEP SRES.
   destruct tl as [ta a]. destruct ta.
-  4: { exfalso. apply NORES. desf. }
-  all: destruct STEP as [STEP [AA BB]].
-  all: split; splits.
-  all: try now (eapply iord_coherent_equiv_wo_reserved; [|apply BB]; basic_solver).
-  all: try now (eapply iord_coherent_equiv_wo_reserved; [|apply AA]; basic_solver).
-  all: apply seq_eqv_l in STEP; destruct STEP as [TT STEP].
-  all: apply seq_eqv_l; split.
-  all: try now (generalize TT; unfolder; ins; desf; tauto). 
-  all: rewrite STEP.
-  all: split; unfolder; ins; desf; ins; splits; auto.
+  4: { left. apply set_extensionality.
+       erewrite iiord_step_incl with (tc1:=tc1) (tc2:=tc2); eauto.
+       rewrite set_minus_union_l. split; [basic_solver|].
+       unionL; clear; basic_solver. }
+  all: right.
+  all: apply iiord_fixed_reserve_step_minus_reserved; auto.
   all: intros HH; inv HH.
 Qed.
 
@@ -378,6 +426,26 @@ Proof using.
 Qed.
 
 (* TODO: move *)
+Lemma isim_clos_step_fixed_reserve s tl tc1 tc2
+  (SRES : s ⊆₁ action ↓₁ (eq ta_reserve))
+  (STEP : isim_clos_step G sc tl tc1 tc2) :
+  (isim_clos_step G sc tl)^? ((tc1 \₁ action ↓₁ (eq ta_reserve)) ∪₁ s)
+                             ((tc2 \₁ action ↓₁ (eq ta_reserve)) ∪₁ s).
+Proof using.
+  clear -STEP SRES.
+  unfold isim_clos_step in *. desf.
+  all: try now (apply iiord_step_fixed_reserved; auto).
+  all: right.
+  all: destruct STEP as [AA [y [STEP0 STEP1]]].
+  all: split; auto.
+  all: eexists; split.
+  all: try now eapply iiord_fixed_reserve_step_minus_reserved; eauto.
+  destruct STEP1 as [z [STEP1 STEP2]].
+  eexists; split.
+  all: try now eapply iiord_fixed_reserve_step_minus_reserved; eauto.
+Qed.
+
+(* TODO: move *)
 Lemma isim_clos_step_minus_reserved tl tc1 tc2
   (STEP : isim_clos_step G sc tl tc1 tc2) :
   (isim_clos_step G sc tl)^? (tc1 \₁ action ↓₁ (eq ta_reserve))
@@ -396,13 +464,118 @@ Proof using.
   all: try now eapply iiord_no_reserve_step_minus_reserved; eauto.
 Qed.
 
+(* TODO: move *)
+Section OnlyInitReserve.
+Definition reserve_init_clos tc := 
+  (tc \₁ action ↓₁ (eq ta_reserve)) ∪₁ eq ta_reserve <*> (acts_set G ∩₁ is_init).
+
+Add Parametric Morphism : reserve_init_clos with signature
+  set_subset ==> set_subset as reserve_init_clos_mori.
+Proof using.
+  clear. intros a b IN.
+  unfold reserve_init_clos. now rewrite IN.
+Qed.
+
+Add Parametric Morphism : reserve_init_clos with signature
+  set_equiv ==> set_equiv as reserve_init_clos_more.
+Proof using.
+  clear. intros a b [AA BB].
+  now split; [rewrite AA|rewrite BB].
+Qed.
+
+Lemma reserve_init_clos_union a b :
+  reserve_init_clos (a ∪₁ b) ≡₁ reserve_init_clos a ∪₁ reserve_init_clos b.
+Proof using. clear. unfold reserve_init_clos. basic_solver 10. Qed.
+
+Lemma reserve_init_clos_init_tls : reserve_init_clos (init_tls G) ≡₁ init_tls G.
+Proof using.
+  clear.
+  unfold reserve_init_clos, init_tls.
+  rewrite !set_pair_union_l, !set_minus_union_l.
+  split; unionL.
+  all: try basic_solver.
+  { do 4 unionR left. unfold set_pair. unfolder. ins. do 2 desf. }
+  { do 3 unionR left. unfold set_pair. unfolder. ins. do 2 desf.
+    right. splits; eauto. intros HH; inv HH. }
+  unionR left -> right.
+  unfold set_pair, is_ta_propagate_to_G. unfolder. ins. do 2 desf.
+  splits; eauto. intros HH; inv HH.
+Qed.
+  
+Lemma reserve_init_clos_tls_coherent
+  tc (TCOH : tls_coherent G tc) :
+  tls_coherent G (reserve_init_clos tc).
+Proof using.
+  destruct TCOH as [AA BB].
+  unfold reserve_init_clos. constructor.
+  { rewrite <- AA. unfold init_tls. clear.
+    rewrite !set_pair_union_l. unfold set_pair, is_ta_propagate_to_G.
+    unfolder. ins. desf; desf; ins; eauto 10.
+    all: now left; split; [|intros HH; inv HH]; eauto 20. }
+  unionL.
+  { transitivity tc; eauto with hahn. basic_solver. }
+  unionR left. unfold init_tls.
+  rewrite !set_pair_union_l. eauto with hahn.
+Qed.
+
+Lemma reserve_init_clos_sim_coherent
+  tc (SCOH : sim_coherent G tc) :
+  sim_coherent G (reserve_init_clos tc).
+Proof using.
+  unfold reserve_init_clos. red.
+  split.
+  { unfold sim_clos. eauto with hahn. }
+  unfold sim_clos.
+  apply set_subset_union_l; split.
+  apply set_subset_union_l; split; eauto with hahn.
+  all: unionR left.
+  all: rewrite set_minusE at 2.
+  all: apply set_subset_inter_r; split.
+  all: try now (unfold rmw_clos, rel_clos, set_pair; unfolder; ins; do 2 desf).
+  all: transitivity (sim_clos G tc); try now apply SCOH.
+  all: unfold sim_clos.
+  1: transitivity (rmw_clos G tc); eauto with hahn.
+  2: transitivity (rel_clos G tc); eauto with hahn.
+  all: unfold rmw_clos, rel_clos.
+  all: apply set_pair_mori; eauto with hahn.
+  all: autorewrite with cir_simplify.
+  all: clear; basic_solver.
+Qed.
+
+Lemma reserve_init_clos_sim_clos_step_rt :
+  sim_clos_step G sc ⊆ reserve_init_clos ↓ (sim_clos_step G sc)^?.
+Proof using.
+  clear.
+  intros tc tc' STEP. red.
+  clear -STEP.
+  destruct STEP as [[tll STEP] [SCOH SCOH']].
+  unfold reserve_init_clos.
+  eapply isim_clos_step_fixed_reserve in STEP.
+  { destruct STEP as [EQ|STEP]; [now left; apply EQ|right].
+    split.
+    2: now split; apply reserve_init_clos_sim_coherent.
+    exists tll; auto. }
+  unfold set_pair. unfolder. ins. do 2 desf.
+Qed.
+
+Lemma reserve_init_clos_sim_clos_steps_rt :
+  (sim_clos_step G sc)^* ⊆ reserve_init_clos ↓ (sim_clos_step G sc)^*.
+Proof using.
+  clear.
+  rewrite reserve_init_clos_sim_clos_step_rt at 1.
+  rewrite map_rel_crt.
+  now rewrite rt_of_cr.
+Qed.
+
+End OnlyInitReserve.
+
 Lemma isim_clos_step2ext_isim_trav_step_rt tc1 tc2 thread tl
   (INIT1 : init_tls G ⊆₁ tc1)
+  (RESEMPTC2 : reserved tc2 ⊆₁ acts_set G ∩₁ is_init)
   (TCOH2 : tls_coherent G tc2)
   (SCOH1 : sim_coherent G tc1)
   (SCOH2 : sim_coherent G tc2)
-  (RESEMPTC2 : reserved tc2 ⊆₁ acts_set G ∩₁ is_init)
-  (STEP : isim_clos_step G sc tl tc1 tc2)
+  (STEP  : isim_clos_step G sc tl tc1 tc2)
   (TLTOTHREAD : match tl with
                 | [] => False
                 | a :: tl => thread = ta_label2thread a
